Implement a little bit more of that interface

providers/evercrypt/fst/EverCrypt.Hash.fst
@@ -10,13 +10,38 @@ module M = LowStar.Modifies
 open LowStar.BufferOps
 open FStar.Integers
 
+#reset-options "--using_facts_from '* -Hacl -Spec'"
+
 let uint32_p = B.buffer uint_32
 let uint64_p = B.buffer uint_64
 
 noeq
 type state_s =
-| SHA256_Hacl: uint32_p -> state_s
-| SHA256_Vale: uint32_p -> state_s
-| SHA384_Hacl: uint64_p -> state_s
+| SHA256_Hacl: p:uint32_p{ B.length p = 8 } -> state_s
+| SHA256_Vale: p:uint32_p{ B.length p = 8 } -> state_s
+| SHA384_Hacl: p:uint64_p{ B.length p = 8 } -> state_s
 
- 
+let invariant_s _ _ =
+  True
+
+let footprint_s (s: state_s): GTot M.loc =
+  match s with
+  | SHA256_Hacl p -> M.loc_buffer p
+  | SHA256_Vale p -> M.loc_buffer p
+  | SHA384_Hacl p -> M.loc_buffer p
+
+let alg_of_s = function
+  | SHA256_Hacl _ | SHA256_Vale _ ->
+      SHA256
+  | SHA384_Hacl _ ->
+      SHA384
+
+let repr s h: GTot _ =
+  let s = B.get h s 0 in
+  match s with
+  | SHA256_Hacl p ->
+      B.as_seq h p
+  | SHA256_Vale p ->
+      B.as_seq h p
+  | SHA384_Hacl p ->
+      B.as_seq h p
